slight refactoring of BaseSystem

src/Galois/BaseSystem.v
@@ -1,28 +1,57 @@
 Require Import List.
 Require Import ZArith.ZArith ZArith.Zdiv.
+  Require Import Omega.
+
+Lemma nth_error_map : forall A B (f:A->B) xs i y,
+  nth_error (map f xs) i = Some y ->
+  exists x, nth_error xs i = Some x /\ f x = y.
+Admitted.
+
+Lemma nth_error_seq : forall start len i,
+  nth_error (seq start len) i =
+  if lt_dec i len
+  then Some (start + i)
+  else None.
+Admitted.
+
+Lemma nth_error_length_error : forall A (xs:list A) i, nth_error xs i = None ->
+  i >= length xs.
+Admitted.
 
 Local Open Scope Z.
 
-Module Type BaseCoefs.
-  (* lists coefficients of digits and the digits themselves always have the
-  * LEAST significant position first. *)
-  Definition coefs : Type := list Z.
+Lemma pos_pow_nat_pos : forall x n, 
+  Z.pos x ^ Z.of_nat n > 0.
+Admitted.
 
-  Parameter base : coefs.
-  Axiom base_positive : forall b, In b base -> b > 0. (* nonzero would probably work too *)
+Module Type BaseCoefs.
+  (** [BaseCoefs] represent the weights of each digit in a positional number system, with the weight of least significant digit presented first. The following requirements on the base are preconditions for using it with BaseSystem. *)
+  Parameter base : list Z.
+  Axiom base_positive : forall b, In b base -> b > 0. (* nonzero would probably work too... *)
   Axiom base_good :
-    forall i j,
+    forall i j, (i+j < length base)%nat ->
     let b := nth_default 0 base in
     let r := (b i * b j) / b (i+j)%nat in
     b i * b j = r * b (i+j)%nat.
 End BaseCoefs.
 
 Module BaseSystem (Import B:BaseCoefs).
+  (** [BaseSystem] implements an constrained positional number system.
+      A wide variety of bases are supported: the base coefficients are not
+      required to be powers of 2, and it is NOT necessarily the case that
+      $b_{i+j} = b_j b_j$. Implementations of addition and multiplication are
+      provided, with focus on near-optimal multiplication performance on
+      non-trivial but small operands: maybe 10 32-bit integers or so. This
+      module does not handle carries automatically: if no restrictions are put
+      on the use of a [BaseSystem], each digit is unbounded. This has nothing
+      to do with modular arithmetic either.
+  *)
   Definition digits : Type := list Z.
 
   Definition accumulate p acc := fst p * snd p + acc.
-  Definition decode bs u  := fold_right accumulate 0 (combine u bs).
-  Hint Unfold decode accumulate.
+  Definition decode' bs u  := fold_right accumulate 0 (combine u bs).
+  Definition decode := decode' base.
+  Hint Unfold decode' accumulate.
 
 	Fixpoint add (us vs:digits) : digits :=
 		match us,vs with
@@ -30,15 +59,15 @@ Module BaseSystem (Import B:BaseCoefs).
 			| _, nil => us
 			| _, _ => vs
 		end.
-  Local Infix ".+" := add (at level 50).
+  Infix ".+" := add (at level 50).
 
-  Lemma add_rep : forall bs us vs, decode bs (add us vs) = decode bs us + decode bs vs.
+  Lemma add_rep : forall bs us vs, decode' bs (add us vs) = decode' bs us + decode' bs vs.
   Proof.
-    unfold decode, accumulate.
+    unfold decode', accumulate.
     induction bs; destruct us; destruct vs; auto; simpl; try rewrite IHbs; ring.
   Qed.
 
-  Lemma decode_nil : forall bs, decode bs nil = 0.
+  Lemma decode_nil : forall bs, decode' bs nil = 0.
     auto.
   Qed.
 
@@ -50,9 +79,9 @@ Module BaseSystem (Import B:BaseCoefs).
 		end.
 
   Definition mul_each u := map (Z.mul u).
-  Lemma mul_each_rep : forall bs u vs, decode bs (mul_each u vs) = u * decode bs vs.
+  Lemma mul_each_rep : forall bs u vs, decode' bs (mul_each u vs) = u * decode' bs vs.
   Proof.
-    unfold decode, accumulate.
+    unfold decode', accumulate.
     induction bs; destruct vs; auto; simpl; try rewrite IHbs; ring.
   Qed.
 
@@ -61,8 +90,8 @@ Module BaseSystem (Import B:BaseCoefs).
     (b(i) * b(j)) / b(i+j)%nat.
 
   Fixpoint zeros n := match n with O => nil | S n' => 0::zeros n' end.
-  Lemma zeros_rep : forall bs n, decode bs (zeros n) = 0.
-    unfold decode, accumulate.
+  Lemma zeros_rep : forall bs n, decode' bs (zeros n) = 0.
+    unfold decode', accumulate.
     induction bs; destruct n; auto; simpl; try rewrite IHbs; ring.
   Qed.
   Lemma length_zeros : forall n, length (zeros n) = n.
@@ -97,20 +126,20 @@ Module BaseSystem (Import B:BaseCoefs).
   *)
 
   Lemma decode_single : forall n bs x,
-    decode bs (zeros n ++ x :: nil) = nth_default 0 bs n * x.
+    decode' bs (zeros n ++ x :: nil) = nth_default 0 bs n * x.
   Proof.
     induction n; intros; simpl.
-    destruct bs; auto; unfold decode, accumulate, nth_default; simpl; ring.
+    destruct bs; auto; unfold decode', accumulate, nth_default; simpl; ring.
     destruct bs; simpl; auto.
-    unfold decode, accumulate, nth_default in *; simpl in *; auto.
+    unfold decode', accumulate, nth_default in *; simpl in *; auto.
   Qed.
 
-  Lemma peel_decode : forall xs ys x y, decode (x::xs) (y::ys) = x*y + decode xs ys.
+  Lemma peel_decode : forall xs ys x y, decode' (x::xs) (y::ys) = x*y + decode' xs ys.
     intros.
-    unfold decode, accumulate, nth_default in *; simpl in *; ring_simplify; auto.
+    unfold decode', accumulate, nth_default in *; simpl in *; ring_simplify; auto.
   Qed.
 
-  Lemma decode_highzeros : forall xs bs n, decode bs (xs ++ zeros n) = decode bs xs.
+  Lemma decode_highzeros : forall xs bs n, decode' bs (xs ++ zeros n) = decode' bs xs.
     induction xs; intros; simpl; try rewrite zeros_rep; auto.
     destruct bs; simpl; auto.
     repeat (rewrite peel_decode).
@@ -119,9 +148,9 @@ Module BaseSystem (Import B:BaseCoefs).
 
   Lemma mul_bi_single : forall m n x,
     (n + m < length base)%nat ->
-    decode base (mul_bi n (zeros m ++ x :: nil)) = nth_default 0 base m * x * nth_default 0 base n.
+    decode (mul_bi n (zeros m ++ x :: nil)) = nth_default 0 base m * x * nth_default 0 base n.
   Proof.
-    unfold mul_bi.
+    unfold mul_bi, decode.
     destruct m; simpl; ssimpl_list; simpl; intros. {
       rewrite decode_single.
       unfold crosscoef; simpl.
@@ -150,7 +179,7 @@ Module BaseSystem (Import B:BaseCoefs).
       rewrite decode_single.
       unfold crosscoef; simpl; ring_simplify.
       rewrite NPeano.Nat.add_1_r.
-      rewrite base_good.
+      rewrite base_good by auto.
       rewrite Z_div_mult.
       rewrite <- Z.mul_assoc.
       rewrite <- Z.mul_comm.
@@ -158,7 +187,7 @@ Module BaseSystem (Import B:BaseCoefs).
       rewrite <- Z.mul_assoc.
       destruct (Z.eq_dec x 0); subst; try ring.
       rewrite Z.mul_cancel_l by auto.
-      rewrite <- base_good.
+      rewrite <- base_good by auto.
       ring.
 
       apply base_positive.
@@ -173,7 +202,7 @@ Module BaseSystem (Import B:BaseCoefs).
   Qed.
   
   Lemma set_higher : forall bs vs x,
-    decode bs (vs++x::nil) = decode bs vs + nth_default 0 bs (length vs) * x.
+    decode' bs (vs++x::nil) = decode' bs vs + nth_default 0 bs (length vs) * x.
   Proof.
     intros.
     rewrite set_higher'.
@@ -194,12 +223,13 @@ Module BaseSystem (Import B:BaseCoefs).
 
   Lemma mul_bi_rep : forall i vs,
     (i + length vs < length base)%nat ->
-    decode base (mul_bi i vs) = decode base vs * nth_default 0 base i.
+    decode (mul_bi i vs) = decode vs * nth_default 0 base i.
   Proof.
+    unfold decode.
     induction vs using rev_ind; intros; simpl. {
-      unfold mul_bi.
+      unfold mul_bi, decode.
       ssimpl_list; rewrite zeros_rep; simpl.
-      unfold decode; simpl.
+      unfold decode'; simpl.
       ring.
     } {
       assert (i + length vs < length base)%nat as inbounds. {
@@ -228,12 +258,13 @@ Module BaseSystem (Import B:BaseCoefs).
 			| _ => nil
     end.
   Definition mul us := mul' (rev us).
-  Local Infix "#*" := mul (at level 40).
+  Infix "#*" := mul (at level 40).
 
   Lemma mul'_rep : forall us vs,
     (length us + length vs <= length base)%nat ->
-    decode base (mul' (rev us) vs) = decode base us * decode base vs.
+    decode (mul' (rev us) vs) = decode us * decode vs.
   Proof.
+    unfold decode.
     induction us using rev_ind; intros; simpl; try apply decode_nil.
 
     assert (length us + length vs < length base)%nat as inbounds. {
@@ -248,14 +279,96 @@ Module BaseSystem (Import B:BaseCoefs).
     rewrite IHus by (rewrite le_trans; eauto); clear IHus.
     rewrite set_higher.
     rewrite mul_each_rep.
-    rewrite mul_bi_rep by auto.
+    rewrite mul_bi_rep by auto; unfold decode.
     ring.
   Qed.
 
   Lemma mul_rep : forall us vs,
     (length us + length vs <= length base)%nat ->
-    decode base (us #* vs) = decode base us * decode base vs.
+    decode (us #* vs) = decode us * decode vs.
   Proof.
     exact mul'_rep.
   Qed.
 End BaseSystem.
+
+Module Type PolynomialBaseParams.
+  Parameter b1 : positive. (* the value at which the polynomial is evaluated *)
+  Parameter baseLength : nat. (* 1 + degree of the polynomial *)
+End PolynomialBaseParams.
+
+Module PolynomialBaseCoefs (Import P:PolynomialBaseParams) <: BaseCoefs.
+  (** PolynomialBaseCoeffs generates base vectors for [BaseSystem] using the extra assumption that $b_{i+j} = b_j b_j$. *)
+  Definition bi i := (Zpos b1)^(Z.of_nat i).
+  Definition base := map bi (seq 0 baseLength).
+
+  Lemma base_positive : forall b, In b base -> b > 0.
+    unfold base.
+    intros until 0; intro H.
+    rewrite in_map_iff in *.
+    destruct H; destruct H.
+    subst.
+    apply pos_pow_nat_pos.
+  Qed.
+
+  Lemma base_good:
+    forall i j, (i + j < length base)%nat ->
+    let b := nth_default 0 base in
+    let r := (b i * b j) / b (i+j)%nat in
+    b i * b j = r * b (i+j)%nat.
+  Proof.
+    unfold base, nth_default.
+    intros; repeat progress (match goal with
+      | [  |- context[match nth_error ?xs ?i with Some _ => _ | None => _ end ] ] => case_eq (nth_error xs i); intros
+      | [ H: nth_error (map _ _) _ = Some _ |- _ ] => destruct (nth_error_map _ _ _ _ _ _ H); clear H
+      | [ H: _ /\ _ |- _ ] => destruct H
+      | [ H: nth_error (seq _ _) _ = Some _ |- _ ] => rewrite nth_error_seq in H
+      | [ H: context[if lt_dec ?a ?b then _ else _] |- _ ] => destruct (lt_dec a b)
+      | [ H: Some _ = Some _ |- _ ] => injection H; clear H; intros; subst
+      | [ H: None = Some _  |- _ ] => inversion H
+      | [ H: Some _ = None |- _ ] => inversion H
+      | [H: nth_error _ _ = None |- _ ] => specialize (nth_error_length_error _ _ _ H); intro; clear H
+    end); autorewrite with list in *; try omega.
+
+    clear.
+    unfold bi.
+    rewrite Nat2Z.inj_add, Zpower_exp by
+      (replace 0 with (Z.of_nat 0) by auto; rewrite <- Nat2Z.inj_ge; omega).
+    rewrite Z_div_same_full; try ring.
+    rewrite <- Z.neq_mul_0.
+    split; apply Z.pow_nonzero; try apply Zle_0_nat; try solve [intro H; inversion H].
+  Qed.
+End PolynomialBaseCoefs.
+
+Module BasePoly2Degree32Params <: PolynomialBaseParams.
+  Definition b1 := 2%positive.
+  Definition baseLength := 32%nat.
+End BasePoly2Degree32Params.
+
+Import ListNotations.
+
+Module BaseSystemExample.
+  Module BasePoly2Degree32Coefs := PolynomialBaseCoefs BasePoly2Degree32Params.
+  Module BasePoly2Degree32 := BaseSystem BasePoly2Degree32Coefs.
+  Import BasePoly2Degree32.
+
+  Example three_times_two : [1;1;0] #* [0;1;0] = [0;1;1;0;0].
+    compute; reflexivity.
+  Qed.
+
+  (* python -c "e = lambda x: '['+''.join(reversed(bin(x)[2:])).replace('1','1;').replace('0','0;')[:-1]+']'; print(e(19259)); print(e(41781))" *)
+  Definition a := [1;1;0;1;1;1;0;0;1;1;0;1;0;0;1].
+  Definition b := [1;0;1;0;1;1;0;0;1;1;0;0;0;1;0;1].
+  Example da : decode a = 19259.
+    compute. reflexivity.
+  Qed.
+  Example db : decode b = 41781.
+    compute. reflexivity.
+  Qed.
+  Example encoded_ab :
+    a #*b =[1;1;1;2;2;4;2;2;4;5;3;3;3;6;4;2;5;3;4;3;2;1;2;2;2;0;1;1;0;1].
+    compute. reflexivity.
+  Qed.
+  Example dab : decode (a #* b) = 804660279.
+    compute. reflexivity.
+  Qed.
+End BaseSystemExample.
